proof halting state

Spacetalk/Experiment.lean
@@ -1,3 +1,4 @@
+import Aesop
 import Mathlib.Data.Vector.Basic
 import Std.Data.DHashMap.Internal.WF
 
@@ -7,14 +8,12 @@ abbrev Ty := Nat
 
 namespace Arith
   inductive Exp
-    | const : Ty → Exp
     | var : String → Exp
     | plus : Exp → Exp → Exp
 
   abbrev Env := String → Ty
 
   inductive Eval : Env → Exp → Ty → Prop
-    | const : Eval env (.const v) v
     | var : env s = v → Eval env (.var s) v
     | plus : Eval env e1 x
       → Eval env e2 y
@@ -25,37 +24,36 @@ namespace Df
   abbrev Nid := Nat
   abbrev Pid := Nat
 
-  structure Tag where
+  structure Port where
     node : Nid
     port : Pid
   deriving DecidableEq
 
   structure Token where
     val : Ty
-    tag : Tag
+    tag : Port
 
   structure BToken where
     val : Ty
-    tags : List Tag
+    tags : List Port
 
   @[simp]
-  def Nid.fst (n : Nid) : Tag := ⟨n, 0⟩
+  def Nid.fst (n : Nid) : Port := ⟨n, 0⟩
 
   @[simp]
-  def Nid.snd (n : Nid) : Tag := ⟨n, 1⟩
+  def Nid.snd (n : Nid) : Port := ⟨n, 1⟩
 
-  inductive Inp
-    | port
-    | const : Ty → Inp
+  inductive BinOp
+    | plus
 
   inductive NodeOp
-    | input : List Tag → NodeOp
-    | output : Inp → NodeOp
-    | plus : Inp → Inp → List Tag → NodeOp
+    | input : List Port → NodeOp
+    | output : NodeOp
+    | binOp : BinOp → List Port → NodeOp
 
   @[simp]
   def NodeOp.isOutput : NodeOp → Bool
-    | .output _ => true
+    | .output => true
     | _ => false
 
   structure Node where
@@ -64,11 +62,11 @@ namespace Df
 
   abbrev DFG := List Node
 
-  abbrev State := Tag → List Ty
+  abbrev State := Port → List Ty
 
   def State.empty : State := λ _ => []
 
-  def State.pop (s : State) (t : Tag) : State :=
+  def State.pop (s : State) (t : Port) : State :=
     λ t' => if t' = t then (s t).tail else s t'
 
   def State.push (s : State) (tok : Token) : State :=
@@ -77,44 +75,41 @@ namespace Df
   def State.pushAll (s : State) (tok : BToken) : State :=
     tok.tags.foldl (λ s tag => s.push ⟨tok.val, tag⟩) s
 
+  def BinOp.denote : BinOp → Ty → Ty → Ty
+    | plus => HAdd.hAdd
+
   infixl:100 " ↤ " => State.pop
   infixl:100 " ↦ " => State.push
   infixl:100 " ↦↦ " => State.pushAll
 
-  inductive Inp.Step : Inp → Tag → State → State → Ty → Prop
-    | port : (h : s tag ≠ []) → Inp.Step .port tag s (s ↤ tag) ((s tag).head h)
-    | const : Inp.Step (.const v) tag s s v
-
   inductive Node.Step : Node → State → State → Prop
     | input : (h : s nid.fst ≠ [])
       → Node.Step ⟨nid, .input ts⟩ s (s ↤ nid.fst ↦↦ ⟨(s nid.fst).head h, ts⟩)
-    | outputConst : s nid.fst = [] → Node.Step ⟨nid, .output (.const c)⟩ s (s ↦ ⟨c, nid.fst⟩)
-    | plus : Inp.Step i1 nid.fst s1 s2 v1 → Inp.Step i2 nid.snd s2 s3 v
-      → Node.Step ⟨nid, .plus i1 i2 ts⟩ s1 (s3 ↦↦ ⟨v1 + v2, ts⟩)
+    | binOp : {op : BinOp} → (h1 : s nid.fst ≠ []) → (h1 : s nid.snd ≠ [])
+      → Node.Step ⟨nid, .binOp op ts⟩ s (s ↤ nid.fst ↤ nid.snd ↦↦ ⟨op.denote v1 v2, ts⟩)
 
-  inductive DFG.Step : DFG → State → State → Prop
-    | refl : DFG.Step dfg s s
+  inductive DFG.MultiStep : DFG → State → State → Prop
+    | refl : DFG.MultiStep dfg s s
     | step : {dfg : DFG} → {node : Node}
       → node ∈ dfg
       → node.Step s1 s2
-      → DFG.Step dfg s2 s3
-      → DFG.Step dfg s1 s3
+      → DFG.MultiStep dfg s2 s3
+      → DFG.MultiStep dfg s1 s3
 end Df
 
 namespace Compiler
-  abbrev VarMap := List (String × Df.Tag)
+  open Arith Df
+
+  abbrev VarMap := List (String × Port)
 
   structure MarkedDFG where
-    dfg : Df.DFG
+    dfg : DFG
     vars : VarMap
-    ret : Df.Tag
+    ret : Port
 
-  def getRetInp (dfg : Df.DFG) (nid : Df.Nid) : Df.Inp :=
-    match dfg.find? (·.id = nid) with
-    | some ⟨_, .output i⟩ => i
-    | _ => .port
-
-  def mergeVarsAux (g1 : MarkedDFG) : Df.DFG × VarMap → String × Df.Tag → Df.DFG × VarMap :=
+  -- Merge consumers of input nodes that map to the same variable
+  @[simp]
+  def mergeVarsAux (g1 : MarkedDFG) : DFG × VarMap → String × Port → DFG × VarMap :=
     λ (dfg, vars) (s, t2) =>
         match dfg.find? (·.id = t2.node) with
         | some ⟨_, .input ts2⟩ =>
@@ -133,45 +128,38 @@ namespace Compiler
           | none => (dfg, (s, t2) :: vars)
         | _ => (dfg, vars)
 
-  def mergeVars (g1 g2 : MarkedDFG) : Df.DFG × VarMap :=
+  def mergeVars (g1 g2 : MarkedDFG) : DFG × VarMap :=
     g2.vars.foldl (mergeVarsAux g1) (g1.dfg ++ g2.dfg, g1.vars)
 
-  def Df.Node.updateReturn (ret : Df.Tag) (newRet : Df.Tag) (node : Df.Node) : Df.Node :=
+  -- Update the "return" value of a graph to be the port of the new output node
+  def Node.updateReturn (ret : Port) (newRet : Port) (node : Node) : Node :=
     let replace t := if t = ret then newRet else t
     {node with op :=
       match node.op with
       | .input ts => .input (ts.map replace)
-      | .output i => .output i
-      | .plus e1 e2 ts => .plus e1 e2 (ts.map replace)
+      | .output => .output
+      | .binOp op ts => .binOp op (ts.map replace)
     }
 
-  def merge (g1 g2 : MarkedDFG) (nid : Df.Nid)
-    : Df.DFG × VarMap × Df.Inp × Df.Inp :=
+  @[simp]
+  def mergeTwo (g1 g2 : MarkedDFG) (nid : Nid)
+    : DFG × VarMap :=
     let (dfg, vars) := mergeVars g1 g2
 
-    -- Find the input edge of the orignal output nodes
-    let ret1 := getRetInp dfg g1.ret.node
-    let ret2 := getRetInp dfg g2.ret.node
-
     -- Update links to the original output nodes
-    let updateReturn dfg ret := match ret with
-      | .port => dfg.map (Df.Node.updateReturn g1.ret nid.fst)
-      | .const _ => dfg
-    let dfg := updateReturn dfg ret1
-    let dfg := updateReturn dfg ret2
+    let dfg := dfg.map (Node.updateReturn g1.ret nid.fst)
+    let dfg := dfg.map (Node.updateReturn g2.ret nid.snd)
 
     -- Remove all output nodes
-    let dfg := dfg.filter (λ node => match node.op with | .output _ => false | _ => true)
-    (dfg, vars, ret1, ret2)
+    let dfg := dfg.filter (λ node => match node.op with | .output => false | _ => true)
+    (dfg, vars)
 
-  def compileAux (maxNid : Df.Nid) : Arith.Exp → MarkedDFG × Df.Nid
-    | .const c =>
-      let dfg := [⟨maxNid, .output (.const c)⟩]
-      (⟨dfg, [], maxNid.fst⟩, maxNid + 1)
+  @[simp]
+  def compileAux (maxNid : Nid) : Exp → MarkedDFG × Nid
     | .var s =>
       let inpId := maxNid
       let outId := maxNid + 1
-      let dfg := [⟨inpId, .input []⟩, ⟨outId, .output .port⟩]
+      let dfg := [⟨inpId, .input []⟩, ⟨outId, .output⟩]
       let vars := [(s, maxNid.fst)]
       (⟨dfg, vars, outId.fst⟩, maxNid + 2)
     | .plus e1 e2 =>
@@ -179,32 +167,32 @@ namespace Compiler
       let (e2, maxNid) := compileAux maxNid e2
       let plusId := maxNid
       let outId := maxNid + 1
-      let (dfg, vars, i1, i2) := merge e1 e2 plusId
-      let dfg := ⟨plusId, .plus i1 i2 [outId.fst]⟩ :: ⟨outId, .output .port⟩ :: dfg
+      let (dfg, vars) := mergeTwo e1 e2 plusId
+      let dfg := ⟨plusId, .binOp .plus [outId.fst]⟩ :: ⟨outId, .output⟩ :: dfg
       (⟨dfg, vars, outId.fst⟩, maxNid + 2)
 
-  def compile (e : Arith.Exp) : MarkedDFG :=
+  @[simp]
+  def compile (e : Exp) : MarkedDFG :=
     (compileAux 0 e).fst
 
-  def MarkedDFG.initialState (dfg : MarkedDFG) (env : Arith.Env) : Df.State :=
+  def MarkedDFG.initialState (dfg : MarkedDFG) (env : Env) : State :=
     dfg.vars.foldl (λ s (name, tag) => s ↦ ⟨env name, tag⟩) .empty
 
   @[simp]
-  def MarkedDFG.finalState (dfg : MarkedDFG) (v : Ty) : Df.State :=
+  def MarkedDFG.finalState (dfg : MarkedDFG) (v : Ty) : State :=
     λ t => if t = dfg.ret then [v] else []
 
   -- Proofs
 
-  abbrev dfg_id_lt_max (dfg : Df.DFG) (max : Df.Nid) :=
+  abbrev dfg_id_lt_max (dfg : DFG) (max : Nid) :=
     ∀ node ∈ dfg, node.id < max
 
   lemma mergeVarsAux_id_eq :
     node ∈ (mergeVarsAux g1 (dfg, vars) (s, t2)).fst → ∃ node' ∈ dfg, node.id = node'.id := by
     intro h_mem
-    simp_all only [mergeVarsAux]
     aesop
 
-  lemma mergeVars_id_eq {dfg1 dfg2 : MarkedDFG} {node : Df.Node}
+  lemma mergeVars_id_eq {dfg1 dfg2 : MarkedDFG} {node : Node}
     (h_mem : node ∈ (mergeVars dfg1 dfg2).fst)
       : (∃ n1 ∈ dfg1.dfg, node.id = n1.id) ∨ (∃ n2 ∈ dfg2.dfg, node.id = n2.id) := by
     have ⟨n, ⟨h_mem, h_id⟩⟩ : ∃ n ∈ dfg1.dfg ++ dfg2.dfg, node.id = n.id := by
@@ -218,32 +206,24 @@ namespace Compiler
       · exact h_mem
     aesop
 
-  lemma updateReturn_id_eq : (Df.Node.updateReturn ret tag node).id = node.id := by
-    simp only [Df.Node.updateReturn]
+  lemma updateReturn_id_eq : (Node.updateReturn ret tag node).id = node.id := by
+    simp only [Node.updateReturn]
 
-  lemma merge_id_lt_max {dfg1 dfg2 : MarkedDFG} {nid : Df.Nid}
-    (maxId : Df.Nid) (h1 : dfg_id_lt_max dfg1.dfg maxId) (h2: dfg_id_lt_max dfg2.dfg maxId)
-    : dfg_id_lt_max (merge dfg1 dfg2 nid).fst maxId := by
+  lemma merge_id_lt_max {dfg1 dfg2 : MarkedDFG} {nid : Nid}
+    (maxId : Nid) (h1 : dfg_id_lt_max dfg1.dfg maxId) (h2: dfg_id_lt_max dfg2.dfg maxId)
+    : dfg_id_lt_max (mergeTwo dfg1 dfg2 nid).fst maxId := by
     intro node h_mem
     have : (∃ node1 ∈ dfg1.dfg, node.id = node1.id)
            ∨ (∃ node2 ∈ dfg2.dfg, node.id = node2.id) := by
-      simp only [merge] at h_mem
+      simp only [mergeTwo] at h_mem
       have := (List.mem_filter.mp h_mem).left
-      -- TODO: Simplify this big split case
-      split at this
-      · obtain ⟨a_update_ret, ⟨h_mem, heq_update_ret⟩⟩ := List.mem_map.mp this
-        split at h_mem
-        obtain ⟨a_update_vars, ⟨h_mem, heq_update_vars⟩⟩ := List.mem_map.mp h_mem
-        all_goals (have := mergeVars_id_eq h_mem; aesop)
-      · split at this
-        · obtain ⟨a_update_vars, ⟨h_mem, heq_update_vars⟩⟩ := List.mem_map.mp this
-          have := mergeVars_id_eq h_mem
-          aesop
-        · have := mergeVars_id_eq this
-          exact this
+      obtain ⟨a_update_ret, ⟨h_mem, heq_update_ret⟩⟩ := List.mem_map.mp this
+      obtain ⟨a_update_vars, ⟨h_mem, heq_update_vars⟩⟩ := List.mem_map.mp h_mem
+      have := mergeVars_id_eq h_mem
+      aesop
     aesop
 
-  lemma compile_maxId_lt {e : Arith.Exp} {initialMax : Df.Nid}
+  lemma compile_maxId_lt {e : Exp} {initialMax : Nid}
     : initialMax < (compileAux initialMax e).snd := by
     cases e <;> simp [compileAux]
     rename_i e1 e2
@@ -253,14 +233,11 @@ namespace Compiler
     exact compile_maxId_lt
     simp
 
-  lemma compile_id_lt_max {e : Arith.Exp} {initialMax : Df.Nid}
+  lemma compile_id_lt_max {e : Exp} {initialMax : Nid}
     : dfg_id_lt_max (compileAux initialMax e).fst.dfg (compileAux initialMax e).snd := by
     intro node h_mem
     cases e with
-    | const _ =>
-      simp_all [compileAux]
     | var _ =>
-      simp_all only [compileAux]
       aesop
     | plus e1 e2 =>
       simp_all only [compileAux]
@@ -288,30 +265,26 @@ namespace Compiler
   abbrev MarkedDFG.ret_if_output (dfg : MarkedDFG) :=
     ∀ node ∈ dfg.dfg, node.op.isOutput = true → node.id = dfg.ret.node
 
+  abbrev MarkedDFG.output_if_ret (dfg : MarkedDFG) :=
+    ∀ node ∈ dfg.dfg, node.id = dfg.ret.node → node.op.isOutput = true
+
   abbrev MarkedDFG.ret_iff_output (dfg : MarkedDFG) :=
     ∀ node ∈ dfg.dfg, node.id = dfg.ret.node ↔ node.op.isOutput = true
 
-  lemma merge_no_output {dfg1 dfg2 : MarkedDFG} {nid : Df.Nid}
+  lemma merge_no_output {dfg1 dfg2 : MarkedDFG} {nid : Nid}
     : dfg1.ret_if_output → dfg2.ret_if_output
-      → ∀ node ∈ (merge dfg1 dfg2 nid).fst, node.op.isOutput = false := by
-    simp_all only [merge]
+      → ∀ node ∈ (mergeTwo dfg1 dfg2 nid).fst, node.op.isOutput = false := by
     aesop
 
   theorem Nat.succ_lt_false {x : Nat} : x + 1 < x → False := by simp
-  theorem Df.Nid.succ_lt_false {x : Df.Nid} : x + 1 < x → False := Nat.succ_lt_false
+  theorem Nid.succ_lt_false {x : Nid} : x + 1 < x → False := Nat.succ_lt_false
 
-  lemma compileAux_ret_if_output {e : Arith.Exp} {maxId : Df.Nid}
+  lemma compileAux_ret_if_output {e : Exp} {maxId : Nid}
     : (compileAux maxId e).fst.ret_if_output := by
     intro node h_mem
     cases e with
-    | const _ =>
-      simp_all only [Df.NodeOp.isOutput, compile, compileAux]
-      aesop
-    | var _ =>
-      simp_all only [Df.NodeOp.isOutput, compile, compileAux]
-      aesop
+    | var _ => aesop
     | plus e1 e2 =>
-      simp_all only [Df.NodeOp.isOutput, compile, compileAux]
       cases h_mem with
       | head => simp_all
       | tail _ h =>
@@ -323,63 +296,58 @@ namespace Compiler
           have := merge_no_output e1_ih e2_ih node h
           simp_all
 
-  lemma compile_ret_iff_output {e : Arith.Exp} : (compile e).ret_iff_output := by
-    intro node h_mem
-    apply Iff.intro
-    · intro h_ret
-      cases e with
-      | const c =>
-        have : node = ⟨0, .output (.const c)⟩ := by
-          simp only [compile, compileAux, Df.Nid.fst, zero_add, List.mem_singleton, h_mem,
-            and_true] at h_mem
-          exact h_mem
-        rw [this]
-        simp
-      | var _ =>
-        simp_all only [compile, compileAux, zero_add, Df.Nid.fst, List.mem_cons,
-          List.mem_singleton]
-        cases h_mem <;> simp_all
-      | plus e1 e2 =>
-        simp_all only [compile, compileAux, Df.Nid.fst, List.mem_cons, Df.NodeOp.isOutput]
-        cases h_mem with
-        | inl h =>
-          simp_all
+  lemma compile_output_if_ret {e : Exp}
+    : (compile e).output_if_ret := by
+    intro node h_mem h_ret
+    cases h_cases : e with
+    | var _ =>
+      simp_all only [compile, compileAux, zero_add, Nid.fst, List.mem_cons,
+        List.mem_singleton]
+      cases h_mem <;> simp_all
+    | plus e1 e2 =>
+      simp_all only [compile, compileAux, Nid.fst, List.mem_cons, NodeOp.isOutput]
+      cases h_mem with
+      | inl h =>
+        simp_all
+      | inr h =>
+        cases h with
+        | inl h => rw [h]
         | inr h =>
-          cases h with
-          | inl h => rw [h]
-          | inr h =>
-            generalize h_max0 : (compileAux 0 e1).snd = maxId0 at *
-            generalize h_max1 : (compileAux maxId0 e2).snd = maxId1 at *
-            have e1_id_lt_max : dfg_id_lt_max (compileAux 0 e1).fst.dfg maxId0 := by
-              rw [←h_max0]
-              exact compile_id_lt_max
-            have e2_id_lt_max : dfg_id_lt_max (compileAux maxId0 e2).fst.dfg maxId1 := by
-              rw [←h_max1]
-              exact compile_id_lt_max
-            have max0_lt_max1 : maxId0 < maxId1 := by
-              rw [←h_max1]
-              exact compile_maxId_lt
-            have e1_id_lt_max : dfg_id_lt_max (compileAux 0 e1).fst.dfg maxId1 :=
-              λ node h_mem => LT.lt.trans (e1_id_lt_max node h_mem) max0_lt_max1
-            have := merge_id_lt_max maxId1 (nid := maxId1) e1_id_lt_max e2_id_lt_max
-            have := this node h
-            rw [h_ret] at this
-            exfalso
-            exact Df.Nid.succ_lt_false this
-    · exact compileAux_ret_if_output node h_mem
+          generalize h_max0 : (compileAux 0 e1).snd = maxId0 at *
+          generalize h_max1 : (compileAux maxId0 e2).snd = maxId1 at *
+          have e1_id_lt_max : dfg_id_lt_max (compileAux 0 e1).fst.dfg maxId0 := by
+            rw [←h_max0]
+            exact compile_id_lt_max
+          have e2_id_lt_max : dfg_id_lt_max (compileAux maxId0 e2).fst.dfg maxId1 := by
+            rw [←h_max1]
+            exact compile_id_lt_max
+          have max0_lt_max1 : maxId0 < maxId1 := by
+            rw [←h_max1]
+            exact compile_maxId_lt
+          have e1_id_lt_max : dfg_id_lt_max (compileAux 0 e1).fst.dfg maxId1 :=
+            λ node h_mem => LT.lt.trans (e1_id_lt_max node h_mem) max0_lt_max1
+          have := merge_id_lt_max maxId1 (nid := maxId1) e1_id_lt_max e2_id_lt_max
+          have := this node h
+          rw [h_ret] at this
+          exfalso
+          exact Nid.succ_lt_false this
 
-  lemma compile_ret_is_fst {nid : Df.Nid} {e : Arith.Exp}
+  lemma compile_ret_iff_output {e : Exp} : (compile e).ret_iff_output :=
+    λ node h_mem => Iff.intro (compile_output_if_ret node h_mem) (compileAux_ret_if_output node h_mem)
+
+  lemma compile_ret_is_fst {nid : Nid} {e : Exp}
     : (compile e).ret.node = nid → (compile e).ret = nid.fst := by
+    simp only [compile, Nid.fst]
     cases e <;> aesop
 
-  theorem compile_value_correct {e : Arith.Exp} {env : Arith.Env} {v : Ty}
-    : Arith.Eval env e v
-      → (compile e).dfg.Step ((compile e).initialState env) ((compile e).finalState v) :=
+  theorem compile_value_correct {e : Exp} {env : Env} {v : Ty}
+    : Eval env e v
+      → (compile e).dfg.MultiStep ((compile e).initialState env) ((compile e).finalState v) :=
     sorry
 
-  theorem compile_confluence {e : Arith.Exp} {a b c : Df.State}
-    : (compile e).dfg.Step a b → (compile e).dfg.Step a c
-        → ∃ d, (compile e).dfg.Step b d ∧ (compile e).dfg.Step c d
+  theorem compile_confluence {e : Exp} {a b c : State}
+    : (compile e).dfg.MultiStep a b → (compile e).dfg.MultiStep a c
+        → ∃ d, (compile e).dfg.MultiStep b d ∧ (compile e).dfg.MultiStep c d
     | .refl, .refl => ⟨a, .intro .refl .refl⟩
     | .refl, s => ⟨c, .intro s .refl⟩
     | s, .refl => ⟨b, .intro .refl s⟩
@@ -387,8 +355,8 @@ namespace Compiler
       cases n1s <;> cases n2s
       all_goals sorry
 
-  lemma final_state_halts {e : Arith.Exp} {v : Ty}
-    : ∀ s, (compile e).dfg.Step ((compile e).finalState v) s → s = (compile e).finalState v := by
+  lemma final_state_halts {e : Exp} {v : Ty}
+    : ∀ s, (compile e).dfg.MultiStep ((compile e).finalState v) s → s = (compile e).finalState v := by
     intro s step
     cases step with
     | refl => rfl
@@ -397,25 +365,21 @@ namespace Compiler
       | input h =>
         rename_i nid ts
         have : nid.fst = (compile e).ret := by simp at h; exact h
-        have : nid = (compile e).ret.node := (Df.Tag.mk.inj this).left
+        have : nid = (compile e).ret.node := (Port.mk.inj this).left
         have := (compile_ret_iff_output ⟨nid, .input ts⟩ h_mem).mp this
         simp at this
-      | outputConst h =>
-        rename_i nid c
-        simp_all only [MarkedDFG.finalState]
-        have := (compile_ret_iff_output ⟨nid, .output (.const c)⟩ h_mem).mpr (by simp)
-        have : (compile e).ret = nid.fst := by
-          apply compile_ret_is_fst
+      | binOp h1 h2 =>
+        rename_i nid _ _ _ _
+        have : nid.fst ≠ (compile e).ret := by
+          intro h
+          have := (compile_ret_iff_output _ h_mem).mp (Port.mk.inj h).left
           simp_all
-        rw [this] at h
         simp_all
-      | plus is1 is2 =>
-        sorry
 
-  theorem compile_correct {e : Arith.Exp} {env : Arith.Env} {v : Ty}
-    : Arith.Eval env e v
-      → ∀ s, (compile e).dfg.Step ((compile e).initialState env) s
-            → (compile e).dfg.Step s ((compile e).finalState v) := by
+  theorem compile_correct {e : Exp} {env : Env} {v : Ty}
+    : Eval env e v
+      → ∀ s, (compile e).dfg.MultiStep ((compile e).initialState env) s
+            → (compile e).dfg.MultiStep s ((compile e).finalState v) := by
     intro as s ds
     have := compile_confluence ds (compile_value_correct as)
     obtain ⟨w, h⟩ := this
